src/HOL/Inductive.thy
@@ -258,38 +258,6 @@ lemma gfp_mono: "(!!Z. f Z \<le> g Z) ==> gfp f \<le> gfp g"
 
 subsection {* Inductive predicates and sets *}
 
-text {* Inversion of injective functions. *}
-
-constdefs
-  myinv :: "('a => 'b) => ('b => 'a)"
-  "myinv (f :: 'a => 'b) == \<lambda>y. THE x. f x = y"
-
-lemma myinv_f_f: "inj f ==> myinv f (f x) = x"
-proof -
-  assume "inj f"
-  hence "(THE x'. f x' = f x) = (THE x'. x' = x)"
-    by (simp only: inj_eq)
-  also have "... = x" by (rule the_eq_trivial)
-  finally show ?thesis by (unfold myinv_def)
-qed
-
-lemma f_myinv_f: "inj f ==> y \<in> range f ==> f (myinv f y) = y"
-proof (unfold myinv_def)
-  assume inj: "inj f"
-  assume "y \<in> range f"
-  then obtain x where "y = f x" ..
-  hence x: "f x = y" ..
-  thus "f (THE x. f x = y) = y"
-  proof (rule theI)
-    fix x' assume "f x' = y"
-    with x have "f x' = f x" by simp
-    with inj show "x' = x" by (rule injD)
-  qed
-qed
-
-hide const myinv
-
-
 text {* Package setup. *}
 
 theorems basic_monos =
